Reentering dependent type hell, because out-of-bounds values are annoying for induction

Regex/Algorithm/Defs.lean
@@ -8,15 +8,19 @@ inductive Action (α : Type u) : Type u where
   /-- Start a regex match (and maybe finish it). -/
   | regex (r : Regex α) (w : List α) (s : ℕ) (cap : Captures) : Action α
   /-- Wait for matches from the first regex of a concatenation -/
-  | concatWait (q : Regex α) (r : Regex α) (w : List α) (s : ℕ) : Action α
+  | concatWait (r : Regex α) (w : List α) : Action α
   /-- Process the second regex with another match -/
-  | concat (r : Regex α) (w : List α) (s : ℕ) (old new : PartialMatches) : Action α
+  | concat (r : Regex α) (w : List α) (old new : PartialMatches) : Action α
   /-- Wait for matches from the first regex of an alternation -/
   | orWait (r : Regex α) (w : List α) (s : ℕ) (cap : Captures) : Action α
   /-- Concatenate the two lists of matches -/
-  | or (s : ℕ) (fst : PartialMatches) : Action α
-  /-- Filter matches for emptiness -/
-  | filterEmpty (emp : Bool) (s : ℕ) : Action α
+  | or (fst : PartialMatches) : Action α
+  /-- Wait for matches from the first match attempt of a star -/
+  | starWait (t : StarType) (r : Regex α) (w : List α) (s : ℕ) (cap : Captures): Action α
+  /-- Process the star with another match. This looks like `concat`,
+  but has special behavior that it's not worth complicating `concat` for. -/
+  | star (t : StarType) (r : Regex α) (w : List α) (s : ℕ) (cap : Captures)
+    (old new : PartialMatches) : Action α
   /-- Capture a match -/
   | capture (n : ℕ) (s : ℕ) : Action α
   deriving Repr
@@ -34,12 +38,9 @@ def Action.process (ac : Action α) (arg : PartialMatches)
     | .bot => ⟨[], []⟩
     | .empty => ⟨[], [(s, cap)]⟩
     | .unit c => ⟨[], if h : w[s]? = c then [(s + 1, cap)] else []⟩
-    | .concat q r => ⟨[regex q w s cap, concatWait q r w s], []⟩
+    | .concat q r => ⟨[regex q w s cap, concatWait r w], []⟩
     | .or q r => ⟨[regex q w s cap, orWait r w s cap], []⟩
-    | .filterEmpty emp r => ⟨[regex r w s cap, filterEmpty emp s], []⟩
-    | .star t r => match t with
-      | .greedy => ⟨[regex [/(⟨r⟩ •ε | (⟨r⟩ -ε)⟨r⟩*‹t›) | ε/] w s cap], []⟩
-      | .lazy => ⟨[regex [/ε | (⟨r⟩ •ε | (⟨r⟩ -ε)⟨r⟩*‹t›)/] w s cap], []⟩
+    | .star t r => ⟨[regex r w s cap, starWait t r w s cap], []⟩
     | .start => ⟨[], if s = 0 then [(s, cap)] else []⟩
     | .end' => ⟨[], if s = w.length then [(s, cap)] else []⟩
     | .capture n r => ⟨[regex r w s cap, capture n s], []⟩
@@ -47,28 +48,32 @@ def Action.process (ac : Action α) (arg : PartialMatches)
       | none => match d with | .bot => [/⊥/] | .empty => [//]
       | some (cs, ct) => list (w.extract cs ct)
       ) w s cap], []⟩
-  | .concatWait _ r w _ => ⟨if h : arg = []
-    then []
-    else [concat r w ((arg.map Prod.fst).min
-      (by contrapose! h; exact List.map_eq_nil_iff.mp h)) arg []], []⟩
-  | .concat r w s old new => match old with
+  | .concatWait r w => ⟨[concat r w arg []], []⟩
+  | .concat r w old new => match old with
     | [] => ⟨[], new ++ arg⟩
-    | (s', cap) :: old => ⟨[regex r w s' cap, concat r w s old (new ++ arg)], []⟩
-  | .orWait r w s cap => ⟨[regex r w s cap, or s arg], []⟩
-  | .or _ fst => ⟨[], fst ++ arg⟩
-  | .filterEmpty emp s => ⟨[], arg.filter fun (s', _) ↦ (s ≥ s') = emp⟩
+    | (s', cap) :: old => ⟨[regex r w s' cap, concat r w old (new ++ arg)], []⟩
+  | .orWait r w s cap => ⟨[regex r w s cap, or arg], []⟩
+  | .or fst => ⟨[], fst ++ arg⟩
+  | .starWait t r w s cap => ⟨[star t r w s cap arg []], []⟩
+  | .star t r w s cap old new => match old with
+    | [] => ⟨[], match t with
+        | .greedy => new ++ arg ++ [(s, cap)]
+        | .lazy => [(s, cap)] ++ new ++ arg⟩
+    | (s', cap) :: old => ⟨if s < s'
+        then [regex [/⟨r⟩*‹t›/] w s' cap, star t r w s cap old (new ++ arg)]
+        else [star t r w s cap old (new ++ arg ++ [(s', cap)])], []⟩
   | .capture n s => ⟨[], arg.map fun (s', cap) ↦
       (s', cap.update n [(s, s')])⟩
 
-/-- The position associated with an action. Used for position lawfulness proofs -/
-def Action.pos (ac : Action α) : ℕ := match ac with
-  | .regex _ _ s _ => s
-  | .concatWait _ _ _ s => s
-  | .concat _ _ s _ _ => s
-  | .orWait _ _ s _ => s
-  | .or s _ => s
-  | .filterEmpty _ s => s
-  | .capture _ s => s
+--/-- The position associated with an action. Used for position lawfulness proofs -/
+--def Action.pos (ac : Action α) : ℕ := match ac with
+--  | .regex _ _ s _ => s
+--  | .concatWait _ _ _ s => s
+--  | .concat _ _ s _ _ => s
+--  | .orWait _ _ s _ => s
+--  | .or s _ => s
+--  | .filterEmpty _ s => s
+--  | .capture _ s => s
 
 -- Apparently without the dependent argument `w`, the type checker doesn't
 -- realize that `StepResult α` is a monad on `MatchStack α` and won't
